Weidenbach_Book/CDCL_Two_Watched_Literals_List_Watched_Init_Trail_Code.thy
@@ -898,12 +898,11 @@ sepref_definition initialise_VMTF_code
   :: \<open>(list_assn uint32_assn)\<^sup>k *\<^sub>a nat_assn\<^sup>k \<rightarrow>\<^sub>a vmtf_remove_conc\<close>
   supply nat_of_uint32_int32_assn[sepref_fr_rules]
   unfolding initialise_VMTF_def vmtf_cons_def
-  apply (rewrite in "((_, _, _, _), \<hole>)" annotate_assn[where A=\<open>list_assn uint32_nat_assn\<close>])
+  apply (rewrite in "((_, _, _, _), \<hole>)" annotate_assn[where A=\<open>arl_assn uint32_nat_assn\<close>])
   apply (rewrite in "(_, _, _, Some \<hole>)" annotate_assn[where A=\<open>uint32_nat_assn\<close>])
   apply (rewrite in "WHILE\<^sub>T _ _ (_, _, _, \<hole>)" annotate_assn[where A=\<open>option_assn uint32_nat_assn\<close>])
   apply (rewrite in "do {ASSERT _; let _ = \<hole>; _}" annotate_assn[where A=\<open>uint32_nat_assn\<close>])
-  apply (rewrite in \<open>((_, _, _, _), ASSN_ANNOT _ \<hole>)\<close> HOL_list.fold_custom_empty
-   op_list_empty_def[symmetric])
+  apply (rewrite in \<open>((_, _, _, _), ASSN_ANNOT _ \<hole>)\<close> arl.fold_custom_empty)
   apply (rewrite in \<open>let _ = \<hole> in _ \<close> array_fold_custom_replicate op_list_replicate_def[symmetric])
   apply (rewrite in "l_vmtf_ATM 0 \<hole> _" annotate_assn[where A=\<open>option_assn uint32_nat_assn\<close>])
   apply (rewrite in "l_vmtf_ATM 0 _ \<hole>" annotate_assn[where A=\<open>option_assn uint32_nat_assn\<close>])
